$$\begin{aligned}
\frac{\partial }{\partial x_k}\bm{x}^\top A\bm{x}&=\frac{\partial }{\partial x_k}\sum_{i}x_i(A\bm{x})_i\\
&=\frac{\partial }{\partial x_k}\sum_{i}x_i\sum_{j}A_{ij}x_{j}\\
&=\frac{\partial }{\partial x_k}\sum_{i}\sum_{j}A_{ij}x_{i}x_{j}\\
&=\sum_{i}\sum_{j}A_{ij}\frac{\partial }{\partial x_k}(x_{i}x_{j})\\
&=\sum_{i}\sum_{j}A_{ij}(\delta_{jk}x_{i}+\delta_{ik}x_{j})\\
&=\sum_{i}A_{ik}x_{i}+\sum_{j}A_{kj}x_{j}\\
&=(A^\top\bm{x})_{k}+(A\bm{x})_{k}\\
&=\left((A+A^\top)\bm{x}\right)_{k}
\end{aligned}$$
Therefore, 
$$\frac{\partial }{\partial \bm{x}}\bm{x}^\top A\bm{x}=(A+A^\top)\bm{x}$$
Here, 
$$\delta_{ij}=\begin{cases}
1 & \rm{if}\ i=j\\
0 & \rm{otherwise}\\
\end{cases}$$